Makefile
@@ -4,7 +4,6 @@ COQC= coqc -Q . Elo
 
 main:
 	$(COQC) Array.v
-	$(COQC) Mem.v
 	$(COQC) Map.v
 	$(COQC) Core0.v
 
